\begin{Lemma}
    $\mathtt{euclidean\_norm(x, y, z) = euclidean\_norm(euclidean\_norm(x, y), z)}$
\end{Lemma}

\begin{solution}
    $\mathtt{euclidean\_norm(x, y, z)}$ is a ternary operation with the signature
    $$\mathtt{euclidean\_norm :: double \times double \times double \rightarrow double}$$
    With currying, the signature becomes
    $$\mathtt{euclidean\_norm :: double \rightarrow double \rightarrow double \rightarrow double}$$
    which clearly associates to
    $$\mathtt{euclidean\_norm :: \left(double \rightarrow double \rightarrow double\right) \rightarrow double}$$

    Now, one can un-curry the parenthesized to obtain
    $$\mathtt{euclidean\_norm :: \left(double \times double \rightarrow double\right) \rightarrow double}$$
    Where, now, the parenthesized is simply the binary operation $\mathtt{euclidean\_norm(x, y)}$, which in this case
    can be taken as a partial application of the function $\mathtt{euclidean\_norm(x,y,z)}$ to the arguments
    $\mathtt{x, y}$. So it is possible to "build" a ternary operation from a binary operation.
\end{solution}